dimsum/spec.v
@@ -1,0 +1,480 @@
+From Paco Require Import paco.
+From ITree Require Export ITree ITreeFacts.
+From ITree.Eq Require Import Paco2.
+From dimsum.core Require Export proof_techniques.
+From dimsum.core Require Import axioms.
+
+(** This file is derived from
+https://github.com/DeepSpec/InteractionTrees/blob/4.0.0/theories/Core/ITreeDefinition.v
+This file also contains many useful comments why definitions are set up in this
+particular way.
+*)
+
+Section spec.
+
+  Local Set Primitive Projections.
+
+  Context {EV : TypeEvent} {S : TypeState} {R : TypeState}.
+
+  (** We need to define our own spec language since the itree type
+  lives in a universe that is too large, which means that it cannot be
+  used in the state type of a module. [specF] explicitly only allows
+  choices over Set such that it can stay in a low universe. The
+  universe problems of itree are probably caused by
+  https://gitlab.mpi-sws.org/iris/stdpp/-/issues/80. *)
+  Variant specF {spec : TypeState} : TypeState :=
+  | SRetF (r : R)
+  | STauF (t : spec)
+  | SVisF (e : EV) (t : spec)
+  | SAllF {X : Set} (k : X → spec)
+  | SExistF {X : Set} (k : X → spec)
+  | SGetF (k : S → spec)
+  | SPutF (s : S) (k : spec)
+  .
+
+  CoInductive spec : TypeState := sgo
+  { sobserve : @specF spec }.
+
+End spec.
+
+Declare Scope spec_scope.
+Bind Scope spec_scope with spec.
+Delimit Scope spec_scope with spec.
+
+Arguments specF _ _ _ : clear implicits.
+Arguments spec _ _ _ : clear implicits.
+
+(** An [spec'] is a "forced" [spec]. It is the type of inputs
+    of [sgo], and outputs of [sobserve]. *)
+Notation spec' EV S R := (specF EV S R (spec EV S R)).
+
+Notation SRet x := (sgo (SRetF x)).
+Notation STau t := (sgo (STauF t)).
+Notation SVis e k := (sgo (SVisF e k)).
+Notation SAll k := (sgo (SAllF k)).
+Notation SExist k := (sgo (SExistF k)).
+Notation SGet k := (sgo (SGetF k)).
+Notation SPut s k := (sgo (SPutF s k)).
+
+(** * Functions on spec *)
+
+Module Spec.
+
+Definition subst {EV S : Type} {T U : Type} (k : T -> spec EV S U)
+  : spec EV S T -> spec EV S U :=
+  cofix _subst (u : spec EV S T) : spec EV S U :=
+    match sobserve u with
+    | SRetF r => k r
+    | STauF t => STau (_subst t)
+    | SVisF e k => SVis e (_subst k)
+    | SAllF k => SAll (λ x, _subst (k x))
+    | SExistF k => SExist (λ x, _subst (k x))
+    | SGetF k => SGet (λ x, _subst (k x))
+    | SPutF s k => SPut s (_subst k)
+    end.
+
+Definition bind {EV S : Type} {T U : Type} (u : spec EV S T) (k : T -> spec EV S U)
+  : spec EV S U :=
+  subst k u.
+
+Definition cat {EV S T U V}
+           (k : T -> spec EV S U) (h : U -> spec EV S V) :
+  T -> spec EV S V :=
+  fun t => bind (k t) h.
+
+Notation on_left lr l t :=
+  (match lr with
+  | inl l => t
+  | inr r => SRet r
+  end) (only parsing).
+
+Definition iter {EV S : Type} {R I: Type}
+           (step : I -> spec EV S (I + R)) : I -> spec EV S R :=
+  cofix iter_ i := bind (step i) (fun lr => on_left lr l (STau (iter_ l))).
+
+(** Functorial map ([fmap] in Haskell) *)
+Definition map {EV S R T} (f : R -> T)  (t : spec EV S R) : spec EV S T :=
+  bind t (fun x => SRet (f x)).
+
+(** Ignore the result. *)
+Definition ignore {EV S R} : spec EV S R -> spec EV S unit :=
+  map (fun _ => tt).
+
+(** Infinite taus. *)
+CoFixpoint spin {EV S R} : spec EV S R := STau spin.
+
+(** Repeat a computation infinitely. *)
+Definition forever {EV S R T} (t : spec EV S R) : spec EV S T :=
+  cofix forever_t := bind t (fun _ => STau (forever_t)).
+End Spec.
+
+(** * Derived notions *)
+Definition TRet {EV S R} (x : R) : spec EV S R :=
+  SRet x.
+
+Definition TVis {EV S} (e : EV) : spec EV S unit :=
+  SVis e (SRet tt).
+
+Definition TAll {EV S} (T : Set) : spec EV S T :=
+  SAll (λ x, SRet x).
+Definition TExist {EV S} (T : Set) : spec EV S T :=
+  SExist (λ x, SRet x).
+
+Definition TGet {EV S} : spec EV S S :=
+  SGet (λ x, SRet x).
+Definition TPut {EV S} (s : S) : spec EV S unit :=
+  SPut s (SRet tt).
+
+Definition TUb {EV S R} : spec EV S R :=
+  SAll (λ x : void, match (x : void) with end).
+Definition TNb {EV S R} : spec EV S R :=
+  SExist (λ x : void, match (x : void) with end).
+
+Definition TAssume {EV S} (P : Prop) : spec EV S unit :=
+  SAll (λ x : P, SRet tt).
+Definition TAssert {EV S} (P : Prop) : spec EV S unit :=
+  SExist (λ x : P, SRet tt).
+
+Definition TAssumeOpt {EV S A} (o : option A) : spec EV S A :=
+  if o is Some x then SRet x else TUb.
+Definition TAssertOpt {EV S A} (o : option A) : spec EV S A :=
+  if o is Some x then SRet x else TNb.
+
+Definition TReceive {EV S} {A : Set} (e : A → EV) : spec EV S A :=
+  Spec.bind (TExist A) (λ x, Spec.bind (TVis (e x)) (λ _, TRet x)).
+(** * Notations *)
+
+Module SpecNotations.
+Notation "m ≫= f" := (Spec.bind f m) (at level 60, right associativity) : spec_scope.
+Notation "x ← y ; z" := (Spec.bind y (λ x : _, z%spec))
+  (at level 20, y at level 100, z at level 200,
+  format "x  ←  y ;  '/' z") : spec_scope.
+Notation "' x ← y ; z" := (Spec.bind y (λ x_ : _, match x_ with x => z%spec end))
+  (at level 20, x pattern, y at level 100, z at level 200,
+  format "' x  ←  y ;  '/' z") : spec_scope.
+Notation "x ;; z" := (Spec.bind x (λ _, z%spec))
+  (at level 100, z at level 200, right associativity) : spec_scope.
+Notation "∀ x .. y , z" :=
+  (Spec.bind (TAll _) (λ x, .. (Spec.bind (TAll _) (λ y, z%spec)) ..)) : spec_scope.
+Notation "∃ x .. y , z" :=
+  (Spec.bind (TExist _) (λ x, .. (Spec.bind (TExist _) (λ y, z%spec)) ..)) : spec_scope.
+End SpecNotations.
+
+Import SpecNotations.
+Definition test1 : spec nat nat nat :=
+  '(a, b) ← TRet (1, 2);
+  x ← TRet 3;
+  TRet (3 + x);;
+  TVis x;;
+  ∀ (x : bool) y,
+  ∃ z,
+  if x then x ← TRet 3; TAssert (x = 2);; TUb else
+  if x then x ← TRet 3; TAssume (x = 2);; TNb else
+  x ← TAssumeOpt (Some 1);
+  x ← TAssertOpt (Some x);
+  s ← TGet ;
+  TPut (s + z +1);;
+  (SRet 3;; SRet 3);;
+  SRet (a - y + b).
+(* Print test1. *)
+
+(** * [sobserving] *)
+(** See https://github.com/DeepSpec/InteractionTrees/blob/4.0.0/theories/Eq/Shallow.v *)
+Record sobserving {EV S R1 R2}
+           (eq_ : spec' EV S R1 -> spec' EV S R2 -> Prop)
+           (t1 : spec EV S R1) (t2 : spec EV S R2) : Prop :=
+  sobserving_intros
+  { sobserving_observe : eq_ (sobserve t1) (sobserve t2) }.
+Global Hint Constructors sobserving: core.
+
+Arguments sobserving_observe {_ _ _ _ _ _ _} _.
+
+Section observing_relations.
+
+Context {EV S R : Type}.
+Variable (eq_ : spec' EV S R -> spec' EV S R -> Prop).
+
+Global Instance sobserving_observe_ :
+  Proper (sobserving eq_ ==> eq_) (@sobserve EV S R).
+Proof. intros ? ? []; cbv; auto. Qed.
+
+Global Instance sobserving_sgo : Proper (eq_ ==> sobserving eq_) (@sgo EV S R).
+Proof. intros ???. constructor. simpl. done. Qed.
+
+Global Instance monotonic_sobserving eq_' :
+  subrelation eq_ eq_' ->
+  subrelation (sobserving eq_) (sobserving eq_').
+Proof. intros ? ? ? []; cbv; eauto. Qed.
+
+Global Instance Equivalence_sobserving :
+  Equivalence eq_ -> Equivalence (sobserving eq_).
+Proof.
+  intros []; split; cbv; auto.
+  - intros ? ? []; auto.
+  - intros ? ? ? [] []; eauto.
+Qed.
+
+End observing_relations.
+
+(** * spec_to_itree *)
+Inductive specE (EV S : Type) : Type → Type :=
+| EVis (e : EV) : specE EV S unit
+| EAll (T : Type) : specE EV S T
+| EExist (T : Type) : specE EV S T
+| EGet : specE EV S S
+| EPut (s : S) : specE EV S unit
+.
+Arguments EVis {_ _}.
+Arguments EAll {_ _}.
+Arguments EExist {_ _}.
+Arguments EGet {_ _}.
+Arguments EPut {_ _}.
+
+Definition spec_to_itree {EV S R} : spec EV S R → itree (specE EV S) R :=
+  cofix _spec_to_itree (t : spec EV S R) : itree _ _ :=
+    match sobserve t with
+    | SRetF x => Ret x
+    | STauF t => Tau (_spec_to_itree t)
+    | SVisF e t => Vis (EVis e) (λ _, (_spec_to_itree t))
+    | SAllF t => Vis (EAll _) (λ x, _spec_to_itree (t x))
+    | SExistF t => Vis (EExist _) (λ x, _spec_to_itree (t x))
+    | SGetF t => Vis EGet (λ x, _spec_to_itree (t x))
+    | SPutF s t => Vis (EPut s) (λ _, _spec_to_itree t)
+    end.
+
+Section spec_to_itree.
+  Notation spec_to_itree_ t :=
+    match sobserve t with
+    | SRetF x => Ret x
+    | STauF t => Tau (spec_to_itree t)
+    | SVisF e t => Vis (EVis e) (λ _, (spec_to_itree t))
+    | SAllF t => Vis (EAll _) (λ x, spec_to_itree (t x))
+    | SExistF t => Vis (EExist _) (λ x, spec_to_itree (t x))
+    | SGetF t => Vis EGet (λ x, spec_to_itree (t x))
+    | SPutF s t => Vis (EPut s) (λ _, spec_to_itree t)
+    end.
+
+  Lemma unfold_spec_to_itree_ {EV S R} (t : spec EV S R)
+    : observing eq (spec_to_itree t) (spec_to_itree_ t).
+  Proof. constructor; reflexivity. Qed.
+
+  Lemma unfold_spec_to_itree_eq {EV S R} (t : spec EV S R)
+    : (spec_to_itree t) ≅ (spec_to_itree_ t).
+  Proof. apply observing_sub_eqit; constructor; reflexivity. Qed.
+
+  Lemma unfold_spec_to_itree {EV S R} (t : spec EV S R)
+    : spec_to_itree t ≈ spec_to_itree_ t.
+  Proof. apply observing_sub_eqit; constructor; reflexivity. Qed.
+End spec_to_itree.
+
+Global Instance sobserving_spec_to_itree {EV S R} :
+  Proper (sobserving eq ==> observing eq) (@spec_to_itree EV S R).
+Proof.
+  repeat intro; subst. constructor. unfold observe. cbn.
+  rewrite (sobserving_observe H). reflexivity.
+Qed.
+
+(** * Equivalence *)
+Global Instance spec_equiv {EV S R} : Equiv (spec EV S R) :=
+  λ t1 t2, eutt eq (spec_to_itree t1) (spec_to_itree t2).
+
+Global Instance spec_equiv_rewrite {EV S R} : RewriteRelation (≡@{spec EV S R}) := { }.
+
+Global Instance spec_equiv_equiv {EV S R} : Equivalence (≡@{spec EV S R}).
+Proof.
+  unfold equiv, spec_equiv.
+  constructor.
+  - move => ?. done.
+  - move => ??. done.
+  - move => ??? ->. done.
+Qed.
+
+Global Instance sobserving_sub_equiv EV S R :
+  subrelation (sobserving eq) (≡@{spec EV S R}).
+Proof. move => ?? Heq. rewrite /equiv/spec_equiv. by rewrite Heq. Qed.
+
+Global Instance spec_equiv_proper {EV S R} RR `{!Reflexive RR} :
+  Proper ((≡) ==> eutt RR) (@spec_to_itree EV S R).
+Proof. unfold equiv, spec_equiv. move => ?? ->. done. Qed.
+
+Lemma spec_eta {EV S R} (t : spec EV S R) : t ≡ sgo (sobserve t).
+Proof. apply sobserving_sub_equiv. econstructor. reflexivity. Qed.
+
+Lemma spec_eta_obs {EV S R} (t : spec EV S R) : sobserving eq t (sgo (sobserve t)).
+Proof. done. Qed.
+
+Lemma spec_eta' {EV S R} (ot : spec' EV S R) : ot = sobserve (sgo ot).
+Proof. reflexivity. Qed.
+
+Section spec_equiv_inv.
+
+  Context {EV S R : Type}.
+
+  Notation spec_equiv_ t1_ t2_ :=
+    match sobserve t1_, sobserve t2_ with
+    | SRetF r1, SRetF r2 => r1 = r2
+    | STauF t1, STauF t2 => t1 ≡ t2
+    | SVisF e1 t1, SVisF e2 t2 => e1 = e2 ∧ t1 ≡ t2
+    | @SAllF _ _ _ _ X1 t1, @SAllF _ _ _ _ X2 t2 =>
+         ∃ p : @eq Type X1 X2, pweqeq (≡) p t1 t2
+    | @SExistF _ _ _ _ X1 t1, @SExistF _ _ _ _ X2 t2 =>
+         ∃ p : @eq Type X1 X2, pweqeq (≡) p t1 t2
+    | SGetF t1, SGetF t2 => ∀ x, t1 x ≡ t2 x
+    | SPutF s1 t1, SPutF s2 t2 => s1 = s2 ∧ t1 ≡ t2
+    | STauF t1, _ => t1 ≡ t2_%spec
+    | _, STauF t2 => t1_%spec ≡ t2
+    | _, _ => False
+    end.
+
+  Lemma spec_equiv_inv (t1 t2 : spec EV S R) : t1 ≡ t2 -> spec_equiv_ t1 t2.
+  Proof.
+    rewrite /equiv/spec_equiv => Heq. rewrite !unfold_spec_to_itree in Heq. move: Heq.
+    move Heq1: (sobserve t1) => ot1. move Heq2: (sobserve t2) => ot2.
+    move => /eqit_inv. destruct ot1, ot2 => //=.
+    all: rewrite ?(spec_eta t1) ?Heq1 ?(spec_eta t2) ?Heq2.
+    all: try move => <-; try move => ->.
+    all: try (etrans; [apply unfold_spec_to_itree|done]).
+    all: try (symmetry; etrans; [apply unfold_spec_to_itree|done]).
+    all: clear Heq1 Heq2 => -[p [He Heq]]; simplify_eq/=.
+    all: try pose proof (UIP_refl _ _ p); simplify_eq/=.
+    - naive_solver.
+    - eexists eq_refl => /=. done.
+    - eexists eq_refl => /=. done.
+    - done.
+    - naive_solver.
+  Qed.
+
+End spec_equiv_inv.
+
+(** * Equivalence on spec' *)
+(* TODO: in itrees, this is handled via going. Should we do this as well here? *)
+Global Instance spec'_equiv {EV S R} : Equiv (spec' EV S R) :=
+  λ t1 t2, sgo t1 ≡ sgo t2.
+
+Global Instance sgo_proper {EV S R} :
+  Proper ((≡) ==> (≡)) (@sgo EV S R).
+Proof. move => ???. done. Qed.
+
+Global Instance STauF_proper {EV S R} :
+  Proper ((≡) ==> (≡)) (@STauF EV S R (spec _ _ _)).
+Proof.
+  move => ??. rewrite /equiv/spec'_equiv/equiv/spec_equiv => Heq. rewrite !unfold_spec_to_itree/=.
+  by setoid_rewrite Heq.
+Qed.
+
+Global Instance SVisF_proper {EV S R} :
+  Proper ((=) ==> (≡) ==> (≡)) (@SVisF EV S R (spec _ _ _)).
+Proof.
+  move => ?? -> ??. rewrite /equiv/spec'_equiv/equiv/spec_equiv => Heq. rewrite !unfold_spec_to_itree/=.
+  by setoid_rewrite Heq.
+Qed.
+
+Global Instance SAllF_proper {EV S R} X :
+  Proper (pointwise_relation _ (≡) ==> (≡)) (@SAllF EV S R (spec _ _ _) X).
+Proof.
+  move => ??. rewrite /equiv/spec'_equiv/equiv/spec_equiv => Heq. rewrite !unfold_spec_to_itree/=.
+  by setoid_rewrite Heq.
+Qed.
+
+Global Instance SExistF_proper {EV S R} X :
+  Proper (pointwise_relation _ (≡) ==> (≡)) (@SExistF EV S R (spec _ _ _) X).
+Proof.
+  move => ??. rewrite /equiv/spec'_equiv/equiv/spec_equiv => Heq. rewrite !unfold_spec_to_itree/=.
+  by setoid_rewrite Heq.
+Qed.
+
+Global Instance SGetF_proper {EV S R} :
+  Proper (pointwise_relation _ (≡) ==> (≡)) (@SGetF EV S R (spec _ _ _)).
+Proof.
+  move => ??. rewrite /equiv/spec'_equiv/equiv/spec_equiv => Heq. rewrite !unfold_spec_to_itree/=.
+  by setoid_rewrite Heq.
+Qed.
+
+Global Instance SPutF_proper {EV S R} :
+  Proper ((=) ==> (≡) ==> (≡)) (@SPutF EV S R (spec _ _ _)).
+Proof.
+  move => ?? -> ??. rewrite /equiv/spec'_equiv/equiv/spec_equiv => Heq. rewrite !unfold_spec_to_itree/=.
+  by setoid_rewrite Heq.
+Qed.
+
+(** * Unfolding of functions  *)
+Section unfold.
+  Notation subst_ k u :=
+    match sobserve u with
+    | SRetF r => k%function r
+    | STauF t => STau (Spec.subst k t)
+    | SVisF e t => SVis e (Spec.subst k t)
+    | SAllF t => SAll (λ x, Spec.subst k (t x))
+    | SExistF t => SExist (λ x, Spec.subst k (t x))
+    | SGetF t => SGet (λ x, Spec.subst k (t x))
+    | SPutF s t => SPut s (Spec.subst k t)
+    end.
+
+  Lemma unfold_subst {EV S T U} (k : T → spec EV S U) (u : spec EV S T)
+    : Spec.subst k u ≡ (subst_ k u).
+  Proof. apply sobserving_sub_equiv; constructor; reflexivity. Qed.
+
+  Notation bind_ u k :=
+    match sobserve u with
+    | SRetF r => k%function r
+    | STauF t => STau (Spec.bind t k)
+    | SVisF e t => SVis e (Spec.bind t k)
+    | SAllF t => SAll (λ x, Spec.bind (t x) k)
+    | SExistF t => SExist (λ x, Spec.bind (t x) k)
+    | SGetF t => SGet (λ x, Spec.bind (t x) k)
+    | SPutF s t => SPut s (Spec.bind t k)
+    end.
+
+  Lemma unfold_bind_ {EV S T U} (k : T → spec EV S U) (u : spec EV S T)
+    : sobserving eq (Spec.bind u k) (bind_ u k).
+  Proof. constructor; reflexivity. Qed.
+
+  Lemma unfold_bind {EV S T U} (k : T → spec EV S U) (u : spec EV S T)
+    : Spec.bind u k ≡ (bind_ u k).
+  Proof. apply sobserving_sub_equiv; constructor; reflexivity. Qed.
+
+  Lemma unfold_forever_ {EV S T U} (t : spec EV S T)
+    : sobserving eq (Spec.forever (T:=U) t) (Spec.bind t (λ _, STau (Spec.forever t))).
+  Proof. rewrite /Spec.forever/=. constructor. reflexivity. Qed.
+
+End unfold.
+
+(** * Lemmas about equivalences  *)
+Lemma stau_equiv {EV S R} (t : spec EV S R) :
+  STau t ≡ t.
+Proof. by rewrite /equiv/spec_equiv unfold_spec_to_itree/= tau_eutt. Qed.
+
+Lemma spec_to_itree_bind {EV S R T} (s : spec EV S R) (t : R → spec EV S T) :
+  spec_to_itree (Spec.bind s t) ≈ ITree.bind (spec_to_itree s) (λ x, spec_to_itree (t x)).
+Proof.
+  revert s t. ginit. pcofix IH => s t.
+  rewrite (unfold_spec_to_itree_eq s).
+  (* TODO: Why is this so slow? *)
+  rewrite unfold_bind_.
+  destruct (sobserve s) => /=.
+  1: rewrite bind_ret_l; by apply reflexivity.
+  all: rewrite unfold_spec_to_itree_eq /= Eq.unfold_bind/=.
+  all: gstep; repeat red; simpl; eauto with paco.
+Qed.
+
+Global Instance bind_Proper {EV S T U} :
+  Proper ((≡) ==> pointwise_relation _ (≡) ==> (≡)) (@Spec.bind EV S T U).
+Proof.
+  move => x y Heq1 ?? Heq2.
+  rewrite /equiv/spec_equiv !spec_to_itree_bind Heq1. by setoid_rewrite Heq2.
+Qed.
+
+Lemma spec_bind_bind {EV S R T U} (s : spec EV S R) (k : R → spec EV S U) (h : U → spec EV S T) :
+  Spec.bind (Spec.bind s k) h ≡ Spec.bind s (fun r => Spec.bind (k r) h).
+Proof.
+  rewrite /equiv/spec_equiv !spec_to_itree_bind bind_bind.
+  f_equiv => ?. rewrite spec_to_itree_bind. done.
+Qed.
+
+Lemma unfold_forever {EV S T U} (t : spec EV S T)
+  : (Spec.forever (T:=U) t) ≡ (Spec.bind t (λ _, Spec.forever t)).
+Proof. rewrite {1}unfold_forever_. setoid_rewrite stau_equiv. done. Qed.
+
+Lemma bind_ret_l {EV S R U} (r : R) (k : R -> spec EV S U) :
+  Spec.bind (TRet r) k ≡ (k r).
+Proof. by rewrite unfold_bind. Qed.
